Make hash trait work

examples/traits/hash.rs
@@ -1,3 +1,5 @@
+// https://doc.rust-lang.org/std/hash/index.html
+
 use std::collections::hash_map::DefaultHasher;
 use std::hash::{Hash, Hasher};
 
